Mise à jour de la contribution lc avec les fichiers envoyés par l'auteur
git-svn-id: svn://scm.gforge.inria.fr/svnroot/coq-contribs/trunk@836 0cf17b13-060f-0410-b1b1-c666bec9822a

Mod.v
@@ -6,79 +6,85 @@
 Set Implicit Arguments.
 
 Require Export Monad.
+Require Import Extensionality.
 
-Record Mod (U : Monad) : Type := {
+(** ** Notations *)
+
+Reserved Notation "x >>>= f" (at level 42, left associativity).
+Reserved Notation "x >>>- f" (at level 42, left associativity).
+
+(** ** Definition of module of a monad. *)
+
+Implicit Type X Y Z : Set.
+
+Record Mod (P : Monad) : Type := {
   mod_carrier :> Set -> Set;
-  mbind : forall (X Y: Set) (f : X -> U Y) (x : mod_carrier X),
+  mbind : forall X Y (f : X -> P Y) (x : mod_carrier X),
     mod_carrier Y;
-  mbind_mbind : forall (X Y Z : Set)
-    (f : X -> U Y) (g : Y -> U Z) (x : mod_carrier X),
+  mbind_mbind : forall X Y Z
+    (f : X -> P Y) (g : Y -> P Z) (x : mod_carrier X),
     mbind Z g (mbind Y f x) = mbind Z (fun u => f u >>= g) x;
-  unit_mbind : forall (X : Set) (x : mod_carrier X),
-    mbind X (@unit U X) x = x
+  unit_mbind : forall X (x : mod_carrier X),
+    mbind X (@unit P X) x = x
 }.
 
 Notation "x >>>= f" := (@mbind _ _ _ _ f x).
 
-Hint Rewrite -> mbind_mbind unit_mbind : mod.
+Hint Rewrite mbind_mbind unit_mbind : mod.
 
-Hint Extern 1 (_ = _ :> @mod_carrier _ _ _) =>
-  autorewrite with mod : mod.
+Hint Extern 1 (_ = _ :> @mod_carrier _ _ _) => autorewrite with mod : mod.
 
-Ltac mod :=
-  intros;
-  autorewrite with monad mod;
-  auto with mod monad.
+Ltac mod := intros; autorewrite with monad mod; auto with mod monad.
 
-Definition mmap (U : Monad) (T : Mod U)
-  (X Y : Set) (f : X -> Y) (x : T X) : T Y :=
-  x >>>= fun x => unit U (f x).
+Definition mmap (P : Monad) (T : Mod P)
+  X Y (f : X -> Y) (x : T X) : T Y :=
+  x >>>= fun x => unit P (f x).
 
 Notation "x >>>- f" := (@mmap _ _ _ _ f x).
 
-Definition mlift (U : Monad) (T : Mod U)
-  (X Y : Set) (f : X -> Y) : T X -> T Y :=
-  @mbind U T _ _ (fun x => unit U (f x)).
+Definition mlift (P : Monad) (T : Mod P) X Y (f : X -> Y) : T X -> T Y :=
+  @mbind P T _ _ (fun x => unit P (f x)).
 
-Definition mlift2 (U : Monad) (T : Mod U) (X Y Z : Set)
-  (f : X -> Y -> Z) (a : U X) (b : T Y) : T Z :=
-  b >>>= (fun y => a >>= fun x => unit U (f x y)).
+Definition mlift2 (P : Monad) (T : Mod P) X Y Z
+  (f : X -> Y -> Z) (a : P X) (b : T Y) : T Z :=
+  b >>>= (fun y => a >>= fun x => unit P (f x y)).
 
 Section Mod_Facts.
 
 Variable P : Monad.
 Variable M : Mod P.
 
-Lemma mbind_congr : forall (X Y : Set) (f g : X -> P Y) (x y : M X),
+Lemma mbind_congr : forall X Y (f g : X -> P Y) (x y : M X),
   x = y -> (forall a, f a = g a) -> x >>>= f = y >>>= g.
 Proof.
-intros. subst y. replace g with f. reflexivity. extens. trivial.
+intros. subst y. replace g with f. reflexivity.
+apply extensionality. trivial.
 Qed.
 
 Hint Resolve mbind_congr : mod.
 
-Lemma unit_mbind_match : forall (X : Set) (f : X -> P X) (x : M X),
+Lemma unit_mbind_match : forall X (f : X -> P X) (x : M X),
   (forall a, f a = unit P a) -> x >>>= f = x.
 Proof.
-intros. replace f with (@unit P X). mod. extens. auto.
+intros.
+transitivity (x >>>= @unit P X).
+apply mbind_congr; trivial.
+auto with mod.
 Qed.
 
-Lemma mmap_mbind : forall (X Y Z : Set)
-  (f : X -> P Y) (g : Y -> Z) (x : M X),
+Lemma mmap_mbind : forall X Y Z (f : X -> P Y) (g : Y -> Z) (x : M X),
   x >>>= f >>>- g = x >>>= (fun u => f u >>- g).
 Proof.
 unfold mmap; mod.
 Qed.
 
-Lemma mbind_mmap : forall (X Y Z : Set)
-  (f : X -> Y) (g : Y -> P Z) (x : M X),
+Lemma mbind_mmap : forall X Y Z (f : X -> Y) (g : Y -> P Z) (x : M X),
   x >>>- f >>>= g = x >>>= fun u : X => g (f u).
 Proof.
 unfold mmap. mod.
 Qed.
 
-Lemma mmap_mmap : forall (X Y Z : Set)
-  (f : X -> Y) (g : Y -> Z) (x : M X),
+Lemma mmap_mmap : forall X Y Z (f : X -> Y) (g : Y -> Z) (x : M X),
   x >>>- f >>>- g = x >>>- fun u : X => g (f u).
 Proof.
 unfold mmap. mod.
@@ -87,40 +93,22 @@ Qed.
 End Mod_Facts.
 
 Hint Resolve unit_mbind_match mbind_congr : mod.
-Hint Rewrite -> mmap_mbind mbind_mmap mmap_mmap : mod.
+Hint Rewrite mmap_mbind mbind_mmap mmap_mmap : mod.
 
-Record Mod_Hom (U : Monad) (S T : Mod U) : Type := {
-  mod_hom_carrier :> forall X : Set, S X -> T X;
-  mod_hom_mbind : forall (X Y : Set) (f : X -> U Y) (x : S X),
+Record Mod_Hom (P : Monad) (S T : Mod P) : Type := {
+  mod_hom_carrier :> forall X, S X -> T X;
+  mod_hom_mbind : forall X Y (f : X -> P Y) (x : S X),
     mod_hom_carrier Y (x >>>= f) = mod_hom_carrier X x >>>= f
 }.
 
-Hint Rewrite -> mod_hom_mbind : mod.
-
-Lemma mod_hom_extens : forall (U : Monad)
-  (S T : Mod U) (f g : Mod_Hom S T),
-  (forall X (x : S X), f X x = g X x) -> f = g.
-Proof.
-destruct f as [f Hf1 Hf2]. destruct g as [g Hg1 Hg2].
-simpl. intros.
-cut (f = g).
-destruct 1. replace Hg1 with Hf1. reflexivity.
-apply proof_irrelevance.
-apply extens_dep with (T := fun X : Set => S X -> T X).
-intros X.
-apply extens.
-trivial.
-Qed.
-
-
+Hint Rewrite mod_hom_mbind : mod.
 
 (** ** Tautological module *)
 
-Definition Taut_Mod (U : Monad) : Mod U :=
-  Build_Mod U U (@bind U) (@bind_bind U) (@unit_bind U).
+Definition Taut_Mod (P : Monad) : Mod P :=
+  Build_Mod P P (@bind P) (@bind_bind P) (@unit_bind P).
 
 Coercion Taut_Mod : Monad >-> Mod.
-
 
 (** ** Pull-back module *)
 
@@ -128,17 +116,16 @@ Section Pull_back.
 
 Variable (P Q: Monad) (h : Monad_Hom P Q) (M : Mod Q).
 
-Let bb (X Y : Set) (f : X -> P Y) (x : M X) : M Y :=
+Let bb X Y (f : X -> P Y) (x : M X) : M Y :=
   x >>>= fun u => h Y (f u).
 
-Remark bb_bb : forall (X Y Z : Set)
-  (f : X -> P Y) (g : Y -> P Z) (x : M X),
+Remark bb_bb : forall X Y Z (f : X -> P Y) (g : Y -> P Z) (x : M X),
   bb Z g (bb Y f x) = bb Z (fun u : X => f u >>= g) x.
 Proof.
 unfold bb; mod.
 Qed.
 
-Remark unit_bb : forall (X : Set) (x : M X),
+Remark unit_bb : forall X (x : M X),
   bb X (unit P (X:=X)) x = x.
 Proof.
 unfold bb; mod.
