Quot.v
@@ -5,13 +5,14 @@
 
 Set Implicit Arguments.
 
-Require Export Misc.
+Require Import Extensionality.
 
+Implicit Type X Y Z W : Set.
 
 (** ** Equivalence relations *)
 
-Record Eqv (A : Set) : Type := {
-  eqv_data :> forall x y : A, Prop;
+Record Eqv (X : Set) : Type := {
+  eqv_data :> X -> X -> Prop;
   eqv_rfl : forall x, eqv_data x x;
   eqv_sym : forall x y, eqv_data y x -> eqv_data x y;
   eqv_trs : forall x y z,
@@ -21,7 +22,7 @@ Record Eqv (A : Set) : Type := {
 Hint Immediate eqv_sym.
 Hint Resolve eqv_rfl eqv_trs.
 
-Lemma eq_eqv : forall (A : Set) (r : Eqv A) x y, x = y -> r x y.
+Lemma eq_eqv : forall X (r : Eqv X) x y, x = y -> r x y.
 Proof.
 destruct 1. apply eqv_rfl.
 Qed.
@@ -49,37 +50,83 @@ Axiom class_rel : forall (X : Set) (r : Eqv X) (x y : X),
   x/r = y/r -> r x y.
 Hint Resolve class_rel.
 
-Axiom class_surj : forall (X : Set) (r : Eqv X) (u : X//r),
-  exists a, a/r = u.
-Hint Resolve class_surj.
+Axiom class_ind : forall (X : Set) (r : Eqv X) (P : X // r -> Prop),
+  (forall x : X, P (x / r)) -> forall x : X // r, P x.
 
 Parameter factor : forall (X : Set) (r : Eqv X) Y (f : X -> Y)
   (Hf : forall x y, r x y -> f x = f y),
   X//r -> Y.
 Implicit Arguments factor [X Y].
 
-Axiom factorize : forall X (r : Eqv X) Y (f : X -> Y)
+Axiom factorize : forall (X : Set) (r : Eqv X) (Y : Set) (f : X -> Y)
   (H : forall x y, r x y -> f x = f y),
     forall x ,  factor r f H (x/r) = f x.
 Hint Resolve factorize.
 Hint Rewrite factorize : quotient.
 
-Lemma factor_extens : forall (X : Set) (r : Eqv X) Y
-  (f : X -> Y) (Hf : forall x y, r x y -> f x = f y)
-  (g : X -> Y) (Hg : forall x y, r x y -> g x = g y)
-  (H : f = g),
-  factor r f Hf = factor r g Hg.
+Lemma factor_extens : forall X (r : Eqv X) Y (f g : X -> Y)
+  (Hf : forall x y, r x y -> f x = f y)
+  (Hg : forall x y, r x y -> g x = g y)
+  (H : forall x, f x = g x),
+  forall x, factor r f Hf x = factor r g Hg x.
 Proof.
-destruct 1. replace Hg with Hf.
-reflexivity.
-apply proof_irrelevance.
+intros.
+apply (class_ind (fun x => factor r f Hf x = factor r g Hg x)).
+intros.
+do 2 rewrite factorize. trivial.
 Qed.
+
+Definition frel X Y (r : Eqv Y) (f g : X -> Y) : Prop :=
+  forall x, r (f x) (g x).
+
+Definition feqv X Y (r : Eqv Y) : Eqv (X -> Y).
+Proof.
+intros.
+split with (@frel X Y r);
+  abstract (unfold frel; simpl; trivial; firstorder eauto).
+Defined.
+
+Definition theta' X Y (r : Eqv Y) : (X -> Y) -> (X -> Y // r) :=
+  fun f x => f x / r.
+
+Lemma theta'_compat : forall  X Y (r : Eqv Y) (f g : X -> Y),
+  feqv X r f g -> theta' r f = theta' r g.
+Proof.
+simpl. intros. unfold theta'.
+apply extensionality. auto.
+Qed.
+
+Definition theta X Y (r : Eqv Y) : (X -> Y) // feqv X r -> X -> Y // r :=
+  fun (f : (X -> Y) // feqv X r) (x : X) =>
+    factor (feqv X r) (@theta' X Y r) (@theta'_compat X Y r) f x.
+
+Axiom theta_surj : forall X Y (r : Eqv Y) (f : X -> Y // r),
+  exists h : (X -> Y) // feqv X r, f = theta h.
+
+Lemma lift_fun : forall X Y (r : Eqv Y) (f : X -> Y // r),
+  exists h : X -> Y, f = fun x => h x / r.
+Proof.
+intros.
+destruct (theta_surj f) as [h Hh].
+generalize h Hh. clear h Hh.
+apply (class_ind
+  (fun h => f = theta h -> exists h0 : X -> Y, f = (fun x : X => h0 x / r))).
+intros g Hg.
+exists g.
+subst f.
+apply extensionality.
+unfold theta.
+intros.
+rewrite factorize.
+reflexivity.
+Qed.
+
+Ltac lift_fun f g :=
+  destruct (lift_fun f) as [g Hlift_f]; subst f.
 
 Section Factor1.
 
-Variable (X : Set) (rX : Eqv X).
-Variable (Y : Set) (rY : Eqv Y).
-Variable f : X -> Y.
+Variable (X : Set) (rX : Eqv X) (Y : Set) (rY : Eqv Y) (f : X -> Y).
 Hypothesis Hf : forall x y, rX x y -> rY (f x) (f y).
 
 Definition factor1 : X // rX -> Y // rY.
@@ -100,24 +147,19 @@ Implicit Arguments factor1 [X Y].
 Implicit Arguments factorize1 [X Y].
 Hint Rewrite factorize1 : quotient.
 
-Ltac class x u :=
-  destruct (class_surj x) as [u []]; try clear x.
-
-Lemma factor1_extens : forall X (rX : Eqv X) Y (rY : Eqv Y)
-  (f : X -> Y) (Hf : forall x y, rX x y -> rY (f x) (f y))
-  (g : X -> Y) (Hg : forall x y, rX x y -> rY (g x) (g y))
-  (H : forall x, rY (f x) (g x)) x,
-  factor1 rX rY f Hf x = factor1 rX rY g Hg x.
+Lemma factor1_extens : forall X (rX : Eqv X) Y (rY : Eqv Y) (f g : X -> Y)
+  (Hf : forall x y, rX x y -> rY (f x) (f y))
+  (Hg : forall x y, rX x y -> rY (g x) (g y))
+  (H : forall x, rY (f x) (g x)),
+  forall x, factor1 rX rY f Hf x = factor1 rX rY g Hg x.
 Proof.
-intros. class x u.
-do 2 rewrite factorize1. auto.
+intros. unfold factor1.
+apply factor_extens. auto.
 Qed.
 
 Section Factor2.
 
-Variable (X : Set) (rX : Eqv X).
-Variable (Y : Set) (rY : Eqv Y).
-Variable (Z : Set) (rZ : Eqv Z).
+Variable (X : Set) (rX : Eqv X) (Y : Set) (rY : Eqv Y) (Z : Set) (rZ : Eqv Z).
 Variable f : X -> Y -> Z.
 
 Hypothesis Hf : forall x y z w,
@@ -130,7 +172,11 @@ Defined.
 
 Remark rmk : forall x y, rX x y -> h x = h y.
 Proof.
-unfold h. intros. extens u. class u v.
+unfold h. intros. apply extensionality.
+apply (class_ind
+  (fun x0 =>
+    factor1 rY rZ (f x) (h_subproof x) x0 = factor1 rY rZ (f y) (h_subproof y) x0)).
+intros.
 do 2 rewrite factorize1. auto.
 Qed.
 
@@ -162,20 +208,12 @@ Lemma factor2_extens :
   (H : forall x y, rZ (f x y) (g x y)) x y,
   factor2 rX rY rZ f Hf x y = factor2 rX rY rZ g Hg x y.
 Proof.
-intros. class x u. class y v.
-do 2 rewrite factorize2. auto.
+intros until 1.
+apply (class_ind
+  (fun x => forall (y : Y // rY),
+     factor2 rX rY rZ f Hf x y = factor2 rX rY rZ g Hg x y)).
+intro.
+apply (class_ind
+  (fun y => factor2 rX rY rZ f Hf (x/rX) y = factor2 rX rY rZ g Hg (x/rX) y)).
+intro. do 2 rewrite factorize2. auto.
 Qed.
-
-Lemma lift_fun : forall (X Y : Set) (r : Eqv Y) (f : X -> Y // r),
-  exists h : X -> Y, f = fun x => h x / r.
-Proof.
-intros.
-pose (R := fun x y => f x = y / r).
-destruct (functional_choice R) as [g Hg].
-unfold R. intros.
-class (f x) u. exists u. reflexivity.
-exists g. extens. rewrite Hg. reflexivity.
-Qed.
-
-Ltac lift_fun f g :=
-  destruct (lift_fun f) as [g Hlift_f]; subst f.
