Slc.v
@@ -10,41 +10,58 @@ Set Implicit Arguments.
 
 Require Export Misc.
 
+(** ** Notations *)
+
+Reserved Notation "x == y" (at level 70, no associativity).
+Reserved Notation "x == y :> X"
+  (at level 70, y at next level, no associativity).
+
+Reserved Notation "x //= f" (at level 42, left associativity).
+Reserved Notation "x //- f" (at level 42, left associativity).
+
 Implicit Type X Y Z : Set.
+
+(** ** Inductive datatype of terms *)
 
 Inductive term (X : Set) : Set :=
   | var : X -> term X
   | app : term X -> term X -> term X
   | abs : term (option X) -> term X.
 
-Hint Extern 1 (_ = _ :> term _) =>
-  autorewrite with slc; simpl : slc.
+Hint Extern 1 (_ = _ :> term _) => autorewrite with slc; simpl : slc.
 
-Fixpoint fct (X Y : Set) (f : X -> Y)
-  (x : term X) { struct x } : term Y :=
+Fixpoint fct X Y (f : X -> Y) (x : term X) { struct x } : term Y :=
   match x with
   | var a => var (f a)
   | app x y => app (x //- f) (y //- f)
-  | abs x => abs (x //- (optmap f))
+  | abs x => abs (x //- optmap f)
   end
 where "x //- f" := (@fct _ _ f x).
 
+Lemma fct_fun_cong :
+  forall X (x : term X) Y (f g : X -> Y),
+  (forall u, f u = g u) -> x //- f = x //- g.
+Proof.
+induction x; simpl; auto.
+intros. f_equal. apply IHx.
+destruct u; simpl; auto.
+Qed.
+
 Lemma fct_fct :
-  forall (X Y Z : Set) (f : X -> Y) (g : Y -> Z) (x : term X) ,
+  forall X Y Z (f : X -> Y) (g : Y -> Z) (x : term X) ,
   x //- f //- g = x //- (fun u => g (f u)).
 Proof.
 intros. generalize Y Z f g; clear Y Z f g.
 induction x; simpl; intros; auto.
-congr. rewrite IHx.
-congr; clear x IHx.
-extens x; destruct x; reflexivity.
+f_equal. rewrite IHx.
+apply fct_fun_cong. destruct u; reflexivity.
 Qed.
-Hint Rewrite -> fct_fct : slc.
+Hint Rewrite fct_fct : slc.
 
-Lemma fct_id : forall (X : Set) (f : X -> X) (x : term X),
+Lemma fct_id : forall X (f : X -> X) (x : term X),
   (forall u, f u = u) -> x //- f = x.
 Proof.
-induction x; intros; simpl; congr; auto.
+induction x; intros; simpl; f_equal; auto.
 apply IHx.
 destruct u; simpl; auto.
 Qed.
@@ -64,7 +81,7 @@ Proof.
 unfold shift. intros. rewrite fct_fct. reflexivity.
 Qed.
 
-Hint Rewrite -> shift_fct fct_shift : slc.
+Hint Rewrite shift_fct fct_shift : slc.
 
 Definition comm
   (X Y : Set) (f : X -> term Y) (x : option X) : term (option Y) :=
@@ -73,118 +90,113 @@ Definition comm
   | None => var None
   end.
 
-Remark comm_var : forall X, comm (@var X) = @var (option X).
+Remark comm_var : forall X (u : option X), comm (@var X) u = var u.
 Proof.
-intros; extens.
-destruct x; reflexivity.
+destruct u; reflexivity.
 Qed.
 
-Fixpoint subst (X Y : Set) (f : X -> term Y)
-  (x : term X) { struct x } : term Y :=
+Fixpoint slc_bind X Y (f : X -> term Y) (x : term X) { struct x } : term Y :=
   match x with
   | var x => f x
   | app x y => app (x //= f) (y //= f)
   | abs x => abs (x //= comm f)
   end
-where "x //= f" := (@subst _ _ f x).
+where "x //= f" := (@slc_bind _ _ f x).
 
 Ltac slc :=
   intros;
   repeat first [ progress simpl fct
-               | progress simpl subst
+               | progress simpl slc_bind
                | progress autorewrite with slc ];
   auto with slc.
 
-Lemma subst_var : forall (X Y : Set) (f : X -> term Y) (x : X),
+Lemma slc_bind_fun_cong : forall X (x : term X) Y (f g : X -> term Y),
+  (forall u, f u = g u) -> x //= f = x //= g.
+Proof.
+induction x; simpl; intros; auto.
+f_equal. apply IHx.
+destruct u; simpl; auto.
+Qed.
+
+Lemma slc_bind_var : forall X Y (f : X -> term Y) (x : X),
   var x //=  f = f x.
 Proof.
 reflexivity.
 Qed.
 
-Lemma var_subst : forall X (x : term X),
-  x //= @var X = x.
-Proof.
-induction x; simpl; auto.
-rewrite comm_var.
-auto.
-Qed.
-
-Lemma var_subst_match : forall X (x : term X) (f : X -> term X),
+Lemma slc_var_bind_match : forall X (x : term X) (f : X -> term X),
   (forall u, f u = var u) -> x //= f = x.
 Proof.
-intros; transitivity (x //= @var _).
-congr; extens.
-trivial.
-apply var_subst.
+induction x; simpl; intros; auto.
+f_equal. apply IHx.
+destruct u; simpl. rewrite H. reflexivity. reflexivity.
+Qed.
+Hint Resolve slc_var_bind_match : slc.
+
+Lemma slc_var_bind : forall X (x : term X),
+  x //= @var X = x.
+Proof.
+intros. apply slc_var_bind_match. reflexivity.
 Qed.
 
-Hint Resolve var_subst_match : slc.
-
-Lemma fct_subst : forall (X Y Z : Set)
-  (f : X -> term Y) (g : Y -> Z) (x : term X),
+Lemma slc_fct_bind : forall X Y Z (f : X -> term Y) (g : Y -> Z) (x : term X),
   x //= f //- g = x //= fun u => f u //- g.
 Proof.
 intros. generalize Y Z f g; clear Y Z f g.
-induction x; simpl; intros; congr; auto.
+induction x; simpl; intros; f_equal; auto.
 rewrite IHx.
-congr; clear x IHx.
-extens x; destruct x; slc.
+apply slc_bind_fun_cong.
+destruct u; slc.
 Qed.
-Hint Rewrite -> fct_subst : slc.
+Hint Rewrite slc_fct_bind : slc.
 
-Lemma subst_fct : forall (X Y Z : Set)
-  (f : X -> Y) (g : Y -> term Z) (x : term X),
+Lemma slc_bind_fct : forall X Y Z (f : X -> Y) (g : Y -> term Z) (x : term X),
   x //- f //= g = x //= fun u => g (f u).
 Proof.
 intros; generalize Y Z f g; clear Y Z f g.
-induction x; simpl; intros; congr; auto.
+induction x; simpl; intros; f_equal; auto.
 rewrite IHx.
-congr; clear x IHx.
-extens x; destruct x; reflexivity.
+apply slc_bind_fun_cong. clear x IHx.
+destruct u; reflexivity.
 Qed.
-Hint Rewrite -> subst_fct : slc.
+Hint Rewrite slc_bind_fct : slc.
 
-Lemma shift_subst : forall (X Y : Set) (f : X -> term Y) (x : term X),
+Lemma slc_shift_bind : forall X Y (f : X -> term Y) (x : term X),
   shift (x //= f) = x //= fun a => shift (f a).
 Proof.
-unfold shift.
-intros.
-rewrite fct_subst.
-reflexivity.
+unfold shift. intros.
+rewrite slc_fct_bind. reflexivity.
 Qed.
 
-Lemma subst_shift : forall (X Y : Set)
-  (f : option X -> term Y) (x : term X),
+Lemma slc_bind_shift : forall X Y (f : option X -> term Y) (x : term X),
   shift x //= f = x //= fun a => f (Some a).
 Proof.
-unfold shift.
-intros.
-rewrite subst_fct.
-reflexivity.
+unfold shift. intros.
+rewrite slc_bind_fct. reflexivity.
 Qed.
 
-Hint Rewrite -> shift_subst subst_shift : slc.
+Hint Rewrite slc_shift_bind slc_bind_shift : slc.
 
-Lemma subst_subst : forall (X Y Z : Set)
+Lemma slc_bind_bind : forall X Y Z
   (f : X -> term Y) (g : Y -> term Z) (x : term X),
   x //= f //= g = x //= fun u => f u //= g.
 Proof.
 intros. generalize Y Z f g; clear Y Z f g.
-induction x; simpl; intros; congr; auto.
+induction x; simpl; intros; f_equal; auto.
 rewrite IHx.
-congr; clear x IHx.
-extens x; destruct x; slc.
+apply slc_bind_fun_cong.
+clear x IHx. destruct u; slc.
 Qed.
-Hint Rewrite -> subst_subst : slc.
+Hint Rewrite slc_bind_bind : slc.
 
-Lemma fct_as_subst : forall (X Y : Set) (f : X -> Y) (x : term X),
+Lemma slc_fct_as_bind : forall X Y (f : X -> Y) (x : term X),
   x //- f = x //= (fun a => var (f a)).
 Proof.
 intros. generalize Y f; clear Y f.
 induction x; simpl; intros; auto.
 rewrite IHx; clear IHx.
-congr. congr; clear x.
-extens x; destruct x; reflexivity.
+f_equal. apply slc_bind_fun_cong.
+destruct u; reflexivity.
 Qed.
 
 Definition app1 X (x : term X) : term (option X) :=
@@ -198,14 +210,14 @@ Qed.
 
 Opaque app1.
 
-Lemma fct_app1 : forall (X Y : Set) (f : X -> Y) (x : term X),
+Lemma fct_app1 : forall X Y (f : X -> Y) (x : term X),
   app1 x //- (optmap f) = app1 (x //- f).
 Proof.
 intros.
 do 2 rewrite app1_app.
 simpl. slc.
 Qed.
-Hint Rewrite -> fct_app1 : slc.
+Hint Rewrite fct_app1 : slc.
 
 Lemma app_as_app1 : forall X (x y : term X),
   app x y = app1 x //= default (@var _) y.
@@ -214,47 +226,33 @@ intros. rewrite app1_app. slc.
 symmetry. slc.
 Qed.
 
-Lemma subst_app1 : forall X Y (f : option X -> term Y) (x : term X),
+Lemma slc_bind_app1 : forall X Y (f : option X -> term Y) (x : term X),
   app1 x //= f = app (x //= fun u : X => f (Some u)) (f None).
 Proof.
 intros. rewrite app1_app. simpl. slc.
 Qed.
 
-Hint Rewrite -> subst_app1 : slc.
+Hint Rewrite slc_bind_app1 : slc.
 
-Inductive Beta (X : Set) : term X -> term X -> Prop :=
+Inductive Beta X : term X -> term X -> Prop :=
   | beta_intro : forall (x1 : term (option X)) (x2 : term X),
       Beta (app (abs x1) x2) (x1 //= (default (fun a => var a) x2)).
 
-Lemma beta_intro2 : forall (X : Set)
-  (x1 : term (option X)) (x2 y : term X),
-  x1 //= (default (fun a => var a) x2) = y ->
-    Beta (app (abs x1) x2) y.
+Lemma beta_intro_alt : forall X (x1 : term (option X)) (x2 y : term X),
+  x1 //= (default (fun a => var a) x2) = y -> Beta (app (abs x1) x2) y.
 Proof.
 intros. subst y. apply beta_intro.
-Qed.
-
-Lemma app_abs1 : forall X (x : term (option X)),
-  Beta (app1 (abs x)) x.
-Proof.
-intros. rewrite app1_app. unfold shift. slc.
-apply beta_intro2.
-slc.
-apply var_subst_match.
-destruct u; simpl; reflexivity.
 Qed.
 
 Inductive lcr (X : Set) : term X -> term X -> Prop :=
   | lcr_var : forall a : X, var a == var a
   | lcr_app : forall x1 x2 y1 y2 : term X,
       x1 == x2 -> y1 == y2 -> app x1 y1 == app x2 y2
-  | lcr_abs : forall x y : term (option X),
-      x == y -> abs x == abs y
+  | lcr_abs : forall x y : term (option X), x == y -> abs x == abs y
   | lcr_beta : forall x y : term X, Beta x y -> x == y
   | lcr_eta : forall x : term X, abs (app1 x) == x
   | lcr_sym : forall x y : term X, y == x -> x == y
-  | lcr_trs : forall x y z : term X,
-      lcr x y -> lcr y z -> lcr x z
+  | lcr_trs : forall x y z : term X, lcr x y -> lcr y z -> lcr x z
 where "x == y" := (@lcr _ x y).
 
 Hint Resolve lcr_var lcr_app lcr_abs lcr_eta lcr_beta lcr_trs : slc.
@@ -262,11 +260,7 @@ Hint Immediate lcr_sym : slc.
 
 Lemma lcr_rfl : forall X (x : term X), x == x.
 Proof.
-intros.
-apply lcr_trs with (abs (app1 x)).
-apply lcr_sym.
-apply lcr_eta; reflexivity.
-apply lcr_eta; reflexivity.
+induction x; constructor; auto.
 Qed.
 Hint Resolve lcr_rfl : slc.
 
@@ -276,67 +270,53 @@ intros; subst y; slc.
 Qed.
 Hint Resolve lcr_eq : slc.
 
-Lemma eta_fct : forall (X Y : Set) (f : X -> Y) (x : term X),
+Lemma eta_fct : forall X Y (f : X -> Y) (x : term X),
   abs (app1 x) //- f = abs (app1 (x //- f)).
 Proof.
 induction x; simpl; slc.
 Qed.
 
-Lemma fct_abs : forall (X Y : Set)
-  (f : X -> Y) (x : term (option X)),
-  abs x //- f = abs (x //- optmap f).
-Proof.
-reflexivity.
-Qed.
-
-Lemma lcr_fct : forall (X Y : Set) (f : X -> Y) (x y : term X),
+Lemma lcr_fct : forall X Y (f : X -> Y) (x y : term X),
   x == y -> x //- f == y //- f.
 Proof.
-intros.
-generalize Y f.
-clear Y f.
+intros. generalize Y f. clear Y f.
 induction H; intros; try solve [simpl; slc].
 2: eauto with slc.
 destruct H.
 simpl. slc.
-apply lcr_beta. apply beta_intro2.
-slc. congr.
-extens. destruct x; reflexivity.
+apply lcr_beta. apply beta_intro_alt.
+slc.
+apply slc_bind_fun_cong.
+destruct u; reflexivity.
 Qed.
 
 Hint Resolve lcr_fct : slc.
 
-Lemma eta_subst : forall (X Y : Set)
-  (f : X -> term Y) (x : term X),
+Lemma slc_eta_bind : forall X Y (f : X -> term Y) (x : term X),
   abs (app1 x) //= f = abs (app1 (x //= f)).
 Proof.
 intros. simpl. slc.
 rewrite app1_app. slc.
 Qed.
 
-Lemma lcr_subst_arg : forall (X Y : Set)
-  (f : X -> term Y) (x y : term X),
+Lemma lcr_bind_arg : forall X Y (f : X -> term Y) (x y : term X),
   x == y -> x //= f == y //= f.
 Proof.
 intros. generalize Y f; clear Y f.
 induction H; intros; try solve [simpl; slc].
 3: eauto with slc.
-2: rewrite eta_subst; slc.
-destruct H.
-simpl.
-rewrite subst_subst.
+2: rewrite slc_eta_bind; slc.
+destruct H. simpl.
+rewrite slc_bind_bind.
 apply lcr_beta.
-apply beta_intro2.
-rewrite subst_subst.
-congr.
-clear x1.
-extens x; destruct x; simpl; slc.
+apply beta_intro_alt.
+rewrite slc_bind_bind.
+apply slc_bind_fun_cong.
+destruct u; simpl; slc.
 Qed.
 
-Lemma lcr_subst_fun : forall (X Y : Set)
-  (f g : X -> term Y) (x : term X),
-  (forall u, f u == g u) ->
-  x //= f == x //= g.
+Lemma lcr_bind_fun : forall X Y  (f g : X -> term Y) (x : term X),
+  (forall u, f u == g u) -> x //= f == x //= g.
 Proof.
 intros. generalize Y f g H; clear Y f g H.
 induction x; intros; simpl; slc.
@@ -345,15 +325,13 @@ apply IHx.
 destruct u; simpl; unfold shift; slc.
 Qed.
 
-Lemma lcr_subst : forall (X Y : Set)
-  (f g : X -> term Y) (x y : term X),
-  (forall u, f u == g u) -> x == y ->
-  x //= f == y //= g.
+Lemma lcr_bind : forall X Y (f g : X -> term Y) (x y : term X),
+  (forall u, f u == g u) -> x == y -> x //= f == y //= g.
 Proof.
 intros.
 apply lcr_trs with (x //= g).
-apply lcr_subst_fun; assumption.
-apply lcr_subst_arg; assumption.
+apply lcr_bind_fun; assumption.
+apply lcr_bind_arg; assumption.
 Qed.
 
 Lemma lcr_app1 : forall X (x y : term X),
@@ -361,6 +339,3 @@ Lemma lcr_app1 : forall X (x y : term X),
 Proof.
 intros. do 2 rewrite app1_app. unfold shift. slc.
 Qed.
-
-Notation "x //- f" := (@fct _ _ f x) : lc_scope.
-Notation "x //= f" := (@subst _ _ f x) : lc_scope.
